library/helping/HelpingOnOffResource.v
@@ -1,0 +1,317 @@
+From CRIS.common Require Import CRIS.
+From CRIS.helping Require Import HelpingResource.
+From iris.algebra Require Import gmap_view.
+From iris.bi Require Import big_op.
+
+(* Private authority used only by the HelpingOn/HelpingOff refinement. *)
+#[local] Existing Instance helpingG.
+#[local] Existing Instance helping_inG.
+
+Section protocol.
+  Context `{!crisG Γ Σ α β τ _S _I, !helpingGS}.
+
+  Definition HelpAuth (reqmap : gmap nat help_state) : iProp Σ :=
+    own help_name
+      (None, Some (gmap_view_auth (DfracOwn 1)
+        (to_agree <$> reqmap : gmap nat (agreeR (leibnizO help_state))))).
+
+  Definition help_erasure_init_cond : iProp Σ := HelpAuth ∅.
+
+  Lemma HelpAuth_Help reqmap reqid df st :
+    HelpAuth reqmap -∗ Help reqid df st -∗ ⌜reqmap !! reqid = Some st⌝.
+  Proof.
+    iIntros "● ◯".
+    iCombine "● ◯" gives %[_ WF].
+    rewrite /= -Some_op Some_valid in WF.
+    eapply gmap_view_both_dfrac_valid_discrete in WF as
+      [? [? [_ [WF [_ INCL]]]]].
+    eapply Some_pair_included_r in INCL as INCL.
+    rewrite lookup_fmap_Some in WF.
+    destruct WF as [? [<- Hwf]]. rewrite Hwf.
+    rewrite Some_included_total to_agree_included_L in INCL. clarify.
+  Qed.
+
+  Lemma HelpAuth_issue reqmap reqid N arg :
+    reqmap !! reqid = None →
+    HelpAuth reqmap ==∗
+      HelpAuth (<[reqid := Pend N arg]> reqmap) ∗ HelpPend reqid N arg.
+  Proof.
+    iIntros (Hfresh) "●".
+    rewrite /HelpAuth /HelpPend /Help.
+    iMod (own_update _ _ ((None, _) ⋅ (None, _)) with "●") as "[$ $]".
+    { eapply prod_update; ss.
+      etransitivity; first apply option_update.
+      { eapply (gmap_view_alloc
+          (to_agree <$> reqmap : gmap nat (agreeR (leibnizO help_state)))
+          reqid (DfracOwn 1) (to_agree (Pend N arg))).
+        { rewrite lookup_fmap Hfresh //. }
+        { rewrite dfrac_valid //. }
+        { ss. }
+      }
+      rewrite Some_op -fmap_insert //.
+    }
+    done.
+  Qed.
+
+  Lemma HelpAuth_update reqmap reqid st1 st2 :
+    HelpAuth reqmap -∗ Help reqid (DfracOwn 1) st1 ==∗
+      HelpAuth (<[reqid := st2]> reqmap) ∗
+      Help reqid (DfracOwn 1) st2.
+  Proof.
+    rewrite /HelpAuth /Help. iIntros "● ◯".
+    iPoseProof (HelpAuth_Help with "● ◯") as "%".
+    iMod (own_update_2 with "● ◯") as "[$ $]"; eauto.
+    eapply prod_update; ss. rewrite -!Some_op. eapply option_update.
+    etrans; first eapply gmap_view_replace.
+    { instantiate (1 := to_agree st2). ss. }
+    rewrite fmap_insert //.
+  Qed.
+
+  Lemma HelpAuth_claim reqmap reqid N arg :
+    HelpAuth reqmap -∗ HelpPend reqid N arg ==∗
+      HelpAuth (<[reqid := InProgress]> reqmap) ∗
+      Help reqid (DfracOwn 1) InProgress.
+  Proof. apply HelpAuth_update. Qed.
+
+  Lemma HelpAuth_publish reqmap reqid ret :
+    HelpAuth reqmap -∗ Help reqid (DfracOwn 1) InProgress ==∗
+      HelpAuth (<[reqid := Done ret]> reqmap) ∗ HelpDone reqid ret.
+  Proof.
+    iIntros "● ◯".
+    iMod (HelpAuth_update reqmap reqid InProgress (Done ret) with "● ◯")
+      as "[$ ◯]".
+    by iMod (Help_persist with "◯") as "$".
+  Qed.
+
+  Lemma HelpAuth_observe_done reqmap reqid ret :
+    HelpAuth reqmap -∗ HelpDone reqid ret -∗
+      ⌜reqmap !! reqid = Some (Done ret)⌝.
+  Proof. apply HelpAuth_Help. Qed.
+End protocol.
+
+Section global_protocol.
+  Context `{!crisG Γ Σ α β τ _S _I, !helpingGS}.
+
+  Definition HelpRun (reqmap : gmap nat help_state) : iProp Σ :=
+    ([∗ map] reqid ↦ st ∈ reqmap,
+      match st with
+      | InProgress => Help reqid (DfracOwn 1) InProgress
+      | _ => emp
+      end)%I.
+
+  Definition res_rel (reqmap : gmap nat help_state) (rt rs : Σ) : Prop :=
+    ✓ rs ∧ (Own rs ⊢ |==> Own rt ∗ HelpAuth reqmap ∗ HelpRun reqmap).
+
+  Lemma HelpRun_empty : HelpRun ∅ ⊣⊢ emp.
+  Proof. by rewrite /HelpRun big_sepM_empty. Qed.
+
+  Lemma HelpRun_lookup_acc reqmap reqid st :
+    reqmap !! reqid = Some st →
+    HelpRun reqmap -∗
+      (match st with
+       | InProgress => Help reqid (DfracOwn 1) InProgress
+       | _ => emp
+       end) ∗
+      ((match st with
+        | InProgress => Help reqid (DfracOwn 1) InProgress
+        | _ => emp
+        end) -∗ HelpRun reqmap).
+  Proof.
+    intros Hlookup. rewrite /HelpRun.
+    iIntros "Hrun".
+    iApply (big_sepM_lookup_acc with "Hrun").
+    exact Hlookup.
+  Qed.
+
+  Lemma HelpRun_lookup_in_progress reqmap reqid :
+    reqmap !! reqid = Some InProgress →
+    HelpRun reqmap -∗
+      Help reqid (DfracOwn 1) InProgress ∗
+      (Help reqid (DfracOwn 1) InProgress -∗ HelpRun reqmap).
+  Proof. apply HelpRun_lookup_acc. Qed.
+
+  Lemma HelpRun_delete reqmap reqid st :
+    reqmap !! reqid = Some st →
+    HelpRun reqmap ⊣⊢
+      (match st with
+       | InProgress => Help reqid (DfracOwn 1) InProgress
+       | _ => emp
+       end) ∗ HelpRun (delete reqid reqmap).
+  Proof.
+    intros Hlookup. rewrite /HelpRun.
+    iSplit; iIntros "Hrun".
+    - iDestruct (big_sepM_delete _ reqmap reqid st Hlookup with "Hrun")
+        as "[$ $]".
+    - rewrite (big_sepM_delete _ reqmap reqid st Hlookup). iFrame.
+  Qed.
+
+  Lemma HelpRun_insert reqmap reqid st :
+    HelpRun (<[reqid := st]> reqmap) ⊣⊢
+      (match st with
+       | InProgress => Help reqid (DfracOwn 1) InProgress
+       | _ => emp
+       end) ∗ HelpRun (delete reqid reqmap).
+  Proof.
+    rewrite /HelpRun.
+    iSplit; iIntros "Hrun".
+    - iDestruct (big_sepM_insert_delete with "Hrun") as "[$ $]".
+    - rewrite big_sepM_insert_delete. iFrame.
+  Qed.
+
+  Lemma res_rel_init rt rs :
+    ✓ rs →
+    (Own rs ⊢ |==> Own rt ∗ help_erasure_init_cond) →
+    res_rel ∅ rt rs.
+  Proof.
+    intros Hvalid Hinit. split; first done.
+    iIntros "Hrs".
+    iMod (Hinit with "Hrs") as "[Hrt Hauth]".
+    iModIntro. iFrame.
+    rewrite HelpRun_empty. done.
+  Qed.
+
+  Lemma HelpRun_claim reqmap reqid N arg :
+    HelpAuth reqmap -∗ HelpRun reqmap -∗ HelpPend reqid N arg ==∗
+      HelpAuth (<[reqid := InProgress]> reqmap) ∗
+      HelpRun (<[reqid := InProgress]> reqmap).
+  Proof.
+    iIntros "Hauth Hrun Hpend".
+    iPoseProof (HelpAuth_Help with "Hauth Hpend") as "%Hlookup".
+    iDestruct (HelpRun_delete reqmap reqid (Pend N arg) Hlookup with "Hrun")
+      as "[_ Hrun]".
+    iMod (HelpAuth_claim with "Hauth Hpend") as "[Hauth Htoken]".
+    iModIntro. iFrame "Hauth".
+    rewrite HelpRun_insert /=. iFrame.
+  Qed.
+
+  Lemma HelpRun_publish reqmap reqid ret :
+    reqmap !! reqid = Some InProgress →
+    HelpAuth reqmap -∗ HelpRun reqmap ==∗
+      HelpAuth (<[reqid := Done ret]> reqmap) ∗
+      HelpRun (<[reqid := Done ret]> reqmap) ∗
+      HelpDone reqid ret.
+  Proof.
+    iIntros (Hlookup) "Hauth Hrun".
+    iDestruct (HelpRun_delete reqmap reqid InProgress Hlookup with "Hrun")
+      as "[Htoken Hrun]".
+    iMod (HelpAuth_publish with "Hauth Htoken") as "[Hauth Hdone]".
+    iModIntro. iFrame "Hauth Hdone".
+    rewrite HelpRun_insert /=. iFrame.
+  Qed.
+
+  Lemma res_rel_issue reqmap rt rs reqid N arg :
+    reqmap !! reqid = None →
+    res_rel reqmap rt rs →
+    ∃ rt2, ✓ rt2 ∧
+      (Own rt2 ⊢ |==> HelpPend reqid N arg ∗ Own rt) ∧
+      res_rel (<[reqid := Pend N arg]> reqmap) rt2 rs.
+  Proof.
+    intros Hfresh [Hvalid Hrel].
+    assert (Hissue :
+      Own rs ⊢ |==>
+        (HelpPend reqid N arg ∗ Own rt) ∗
+        (HelpAuth (<[reqid := Pend N arg]> reqmap) ∗
+         HelpRun (<[reqid := Pend N arg]> reqmap))).
+    { iIntros "Hrs".
+      iMod (Hrel with "Hrs") as "[Hrt [Hauth Hrun]]".
+      iMod (HelpAuth_issue reqmap reqid N arg Hfresh with "Hauth")
+        as "[Hauth Hpend]".
+      iModIntro. iSplitL "Hpend Hrt"; first iFrame.
+      iFrame "Hauth".
+      rewrite HelpRun_insert /= (delete_notin reqmap reqid Hfresh). iFrame. }
+    eapply Own_bupd_split in Hissue
+      as [rt2 [rhidden [Hsplit [Hpublic Hhidden]]]]; [|exact Hvalid].
+    exists rt2. split.
+    { eapply (Own_wand_valid rs); last exact Hvalid.
+      iIntros "Hrs".
+      iMod (Hsplit with "Hrs") as "[Hrt2 _]".
+      iModIntro. iFrame. }
+    split.
+    { iIntros "Hrt2".
+      iPoseProof (Hpublic with "Hrt2") as "[Hpend Hrt]".
+      iModIntro. iFrame. }
+    split; first exact Hvalid.
+    iIntros "Hrs".
+    iMod (Hsplit with "Hrs") as "[Hrt2 Hhidden]".
+    iPoseProof (Hhidden with "Hhidden") as "[Hauth Hrun]".
+    iModIntro. iFrame.
+  Qed.
+
+  Lemma res_rel_claim reqmap rt rs reqid N arg rt2 :
+    res_rel reqmap rt rs →
+    (Own rt ⊢ |==> HelpPend reqid N arg ∗ Own rt2) →
+    reqmap !! reqid = Some (Pend N arg) ∧
+    res_rel (<[reqid := InProgress]> reqmap) rt2 rs.
+  Proof.
+    intros [Hvalid Hrel] Hclaim.
+    assert (Hlookup : reqmap !! reqid = Some (Pend N arg)).
+    { eapply (Own_pure_soundness rs); first exact Hvalid.
+      iIntros "Hrs".
+      iMod (Hrel with "Hrs") as "[Hrt [Hauth Hrun]]".
+      iMod (Hclaim with "Hrt") as "[Hpend Hrt2]".
+      iApply (HelpAuth_Help with "Hauth Hpend"). }
+    split; first exact Hlookup.
+    split; first exact Hvalid.
+    iIntros "Hrs".
+    iMod (Hrel with "Hrs") as "[Hrt [Hauth Hrun]]".
+    iMod (Hclaim with "Hrt") as "[Hpend Hrt2]".
+    iMod (HelpRun_claim with "Hauth Hrun Hpend") as "[Hauth Hrun]".
+    iModIntro. iFrame.
+  Qed.
+
+  Lemma res_rel_publish reqmap rt rs reqid ret :
+    reqmap !! reqid = Some InProgress →
+    res_rel reqmap rt rs →
+    ∃ rt2, ✓ rt2 ∧
+      (Own rt2 ⊢ |==> HelpDone reqid ret ∗ Own rt) ∧
+      res_rel (<[reqid := Done ret]> reqmap) rt2 rs.
+  Proof.
+    intros Hlookup [Hvalid Hrel].
+    assert (Hpublish :
+      Own rs ⊢ |==>
+        (HelpDone reqid ret ∗ Own rt) ∗
+        (HelpAuth (<[reqid := Done ret]> reqmap) ∗
+         HelpRun (<[reqid := Done ret]> reqmap))).
+    { iIntros "Hrs".
+      iMod (Hrel with "Hrs") as "[Hrt [Hauth Hrun]]".
+      iMod (HelpRun_publish reqmap reqid ret Hlookup with "Hauth Hrun")
+        as "[Hauth [Hrun Hdone]]".
+      iModIntro. iFrame. }
+    eapply Own_bupd_split in Hpublish
+      as [rt2 [rhidden [Hsplit [Hpublic Hhidden]]]]; [|exact Hvalid].
+    exists rt2. split.
+    { eapply (Own_wand_valid rs); last exact Hvalid.
+      iIntros "Hrs".
+      iMod (Hsplit with "Hrs") as "[Hrt2 _]".
+      iModIntro. iFrame. }
+    split.
+    { iIntros "Hrt2".
+      iPoseProof (Hpublic with "Hrt2") as "[Hdone Hrt]".
+      iModIntro. iFrame. }
+    split; first exact Hvalid.
+    iIntros "Hrs".
+    iMod (Hsplit with "Hrs") as "[Hrt2 Hhidden]".
+    iPoseProof (Hhidden with "Hhidden") as "[Hauth Hrun]".
+    iModIntro. iFrame.
+  Qed.
+
+  Lemma res_rel_observe reqmap rt rs reqid ret rt2 :
+    res_rel reqmap rt rs →
+    (Own rt ⊢ |==> HelpDone reqid ret ∗ Own rt2) →
+    reqmap !! reqid = Some (Done ret) ∧ res_rel reqmap rt2 rs.
+  Proof.
+    intros [Hvalid Hrel] Hobserve.
+    assert (Hlookup : reqmap !! reqid = Some (Done ret)).
+    { eapply (Own_pure_soundness rs); first exact Hvalid.
+      iIntros "Hrs".
+      iMod (Hrel with "Hrs") as "[Hrt [Hauth Hrun]]".
+      iMod (Hobserve with "Hrt") as "[Hdone Hrt2]".
+      iApply (HelpAuth_observe_done with "Hauth Hdone"). }
+    split; first exact Hlookup.
+    split; first exact Hvalid.
+    iIntros "Hrs".
+    iMod (Hrel with "Hrs") as "[Hrt [Hauth Hrun]]".
+    iMod (Hobserve with "Hrt") as "[_ Hrt2]".
+    iModIntro. iFrame.
+  Qed.
+End global_protocol.
